extracted Specs.SeqExt.find (& related) into separate Seq.Find.*

src/Flutterbye.Seq.Find.fsi
@@ -1,0 +1,47 @@
+(*--build-config
+   options:--admit_fsi FStar.Seq;
+   other-files:seq.fsi
+--*)
+
+// $legal:614:
+//
+// Copyright 2015 Michael Lowell Roberts
+//
+// Licensed under the Apache License, Version 2.0 (the "License");
+// you may not use this file except in compliance with the License.
+// You may obtain a copy of the License at
+//
+//     http://www.apache.org/licenses/LICENSE-2.0
+//
+// Unless required by applicable law or agreed to in writing, software
+// distributed under the License is distributed on an "AS IS" BASIS,
+// WITHOUT WARRANTIES OR CONDITIONS OF ANY KIND, either express or implied.
+// See the License for the specific language governing permissions and
+// limitations under the License.
+//
+// ,$
+
+module Flutterbye.Seq.Find
+   open FStar.Seq
+
+   // todo: this isn't working when used from a separate module.
+   val option_get: o: option 'a{is_Some o} -> Tot 'a
+
+   // todo: this should accept an 'a -> bool rather than an 'a.
+   val find: s: seq 'a -> 'a -> Tot (option nat)
+
+   // todo: can this be broken down into simpler lemmas
+   // (e.g. lemma__range and lemma__not_found)?
+   val lemma__basic:
+      s: seq 'a
+      -> a: 'a
+      -> Lemma
+         (requires (True))
+         (ensures
+            ((is_None (find s a) ==>
+               (forall j.
+                  0 <= j && j < length s ==> index s j <> a))
+            /\ (is_Some (find s a) ==>
+                  ((option_get (find s a)) < length s
+                  && a = index s (option_get (find s a))))))
+         [SMTPat (find s a)]
