src/Flutterbye.Seq.Find.fst
@@ -1,0 +1,86 @@
+(*--build-config
+   options:--admit_fsi FStar.Seq;
+   other-files:seq.fsi Flutterbye.Seq.Find.fsi
+--*)
+
+// $legal:614:
+//
+// Copyright 2015 Michael Lowell Roberts
+//
+// Licensed under the Apache License, Version 2.0 (the "License");
+// you may not use this file except in compliance with the License.
+// You may obtain a copy of the License at
+//
+//     http://www.apache.org/licenses/LICENSE-2.0
+//
+// Unless required by applicable law or agreed to in writing, software
+// distributed under the License is distributed on an "AS IS" BASIS,
+// WITHOUT WARRANTIES OR CONDITIONS OF ANY KIND, either express or implied.
+// See the License for the specific language governing permissions and
+// limitations under the License.
+//
+// ,$
+
+module Flutterbye.Seq.Find
+   open FStar.Seq
+
+   // todo: this isn't working when used from another module.
+   let option_get o =
+      match o with
+         | Some a ->
+            a
+
+   val find__loop:
+      s: seq 'a
+      -> 'a
+      -> i: nat{i <= length s}
+      -> c: option nat
+      -> Tot (option nat)
+         (decreases (length s - i))
+   let rec find__loop s a i c =
+      if i < length s then
+         let c' =
+            if is_None c && (a = index s i) then
+               Some i
+            else
+               c in
+         find__loop s a (i + 1) c'
+      else
+         c
+
+   val lemma__basic__loop:
+      s: seq 'a
+      -> a: 'a
+      -> i: nat{i <= length s}
+      -> c: option nat
+      -> Lemma
+         (requires
+            ((is_None c ==>
+               (forall j.
+                  0 <= j && j < i ==> index s j <> a))
+            /\ (is_Some c ==>
+                  ((option_get c) < length s
+                  && a = index s (option_get c)))))
+         (ensures
+            ((is_None (find__loop s a i c) ==>
+               (forall j.
+                  0 <= j && j < length s ==> index s j <> a))
+            /\ (is_Some (find__loop s a i c) ==>
+                  ((option_get (find__loop s a i c)) < length s
+                  && a = index s (option_get (find__loop s a i c))))))
+         (decreases (length s - i))
+   let rec lemma__basic__loop s a i c =
+      if i < length s then
+         let c' =
+            if is_None c && a = index s i then
+               Some i
+            else
+               c in
+         lemma__basic__loop s a (i + 1) c'
+      else
+         ()
+
+   let find s a =
+      find__loop s a 0 None
+   let lemma__basic s a =
+      lemma__basic__loop s a 0 None
